test/Tests.lean
@@ -4,6 +4,7 @@ Released under Apache 2.0 license as described in the file LICENSE.
 -/
 import Tests.Apple
 import Tests.Attempt
+import Tests.Base64Url
 import Tests.Consent
 import Tests.EndToEnd
 import Tests.Digest
